\section{Laplace transform}
Is a generalisation of the Fourier transform and defined as:
$$H(s)=\mathcal{L}\{h(t)\}=\int_{0^-}^{\infty}h(t)e^{ -st }  \, dt \quad\quad s \in\mathbb{C}$$
$s$ is a complex number $s=\sigma+j\omega$ and is identical with Fourier transform, if $s$ is set to $j\omega$.\\
Inverse Laplace tranformation:
$$h(t)=\mathcal{L}^{-1}\{H(t)\}=\frac{1}{2\pi j}\int_{\sigma_{c}-j\infty}^{\sigma_{c}+j\infty} H(s)e^{ st } \, ds $$
\begin{table}[h]
\centering
\begin{tabular}{|c|c|}
\hline
\cellcolor[HTML]{C0C0C0} \textbf{Signal}& \cellcolor[HTML]{C0C0C0}\textbf{Laplace Transform}  \\ \hline
1&$\frac{1}{s}$ \\ \hline
$t^n$&$\frac{n!}{s^{n+1}}$ \\ \hline
$e^{at}$& $\frac{1}{s-a}$ \\ \hline
$\sin(at)$&$\frac{a}{s^2+a^2}$ \\ \hline
$\cos(at)$&$\frac{s}{s^2+a^2}$ \\ \hline
$\cosh(at)$&$\frac{s}{s^2-a^2}$ \\ \hline
$\sinh(at)$&$\frac{a}{s^2-a^2}$ \\ \hline
$e^{at}\cos(\omega t)$&$\frac{s-a}{(s-a)^2+\omega^2}$ \\ \hline
$e^{at}\sin(\omega t)$&$\frac{\omega}{(s-a)^2+\omega^2}$ \\ \hline
\end{tabular}
\end{table}

\subsection{General Formulas}
$$\mathcal{L}\{f(t)\}=F(s)$$
$$\mathcal{L}\{f'\}=s\mathcal{L}\{f\}-f(0)$$
$$\mathcal{L}\{f''\}=s^2\mathcal{L}\{f\}-sf(0)-f'(0)$$
$$\mathcal{L}\{f^n\}=s^n\mathcal{L}\{f\}-s^{n-1}f(0)-\dots -f^{n-1}(0)$$
\subsection{Examples}
\subsubsection{Example 1: Laplace Transform}
Using the Laplace transform, find the solution for the following equation:
$$\frac{\partial^{2}}{\partial t^{2}}y(t)+2\frac{\partial}{\partial t}y(t)+2y(t)=0$$
with initial conditions $y (0) = 1$ and $y' (0) = -1$

\rule{\textwidth}{0.5pt}

Take laplace transform of the equation:
$$s^2Y(s)-sy(0)-y'(0)+2(sY(s)-y(0))+2(Y(s))=0$$
$$s^2Y(s)-s+1+2sY(s)-2+2Y(s)=0$$
$$s^2Y(s)+2sY(s)+2Y(s)=1+s$$
$$(s^2+2s+2)Y(s)=1+s$$
$$Y(s)=\frac{1+s}{(s^2+2s+2)}=\frac{1+s}{((s+1)^2+1)}$$
From table lookup:
$$\mathcal{L}\{e^{at}\cos(\omega t)\}=\frac{s-a}{(s-a)^2+\omega^2}$$
$$a=-1\qquad \omega=1$$
$$y(t)=e^{-t}\cos(t)$$



\subsubsection{Example 2: Transfer Function}
Consider a mass-spring-damper system with the following differential equation:
$$m\overset{..}{x}=-kx-b\overset{.}{x}+f$$

Find the transfer function for the system with input $f$ and output $x$.

\rule{\textwidth}{0.5pt}

$$ms^2X(s)=-kX(s)-bsX(s)+F(s)$$
$$ms^2X(s)+kX(s)+bsX(s)=F(s)$$
$$(ms^2+k+bs)X(s)=F(s)$$
The transfer function is:
$$\frac{X(s)}{F(s)}=\displaystyle\frac{1}{ms^2+k+bs}$$

\subsubsection{Example 3: Differential equation}
Consider:
$$y''(t)+y'(t)=0.5t$$
where $y(0)=0$ and $y'(0)=0$
Use Laplace transform to solve the equation and find $y(t)$

\rule{\textwidth}{0.5pt}

From Laplace transform table:
$$\mathcal{L}\{t\}=\frac{1}{s^2}$$
Laplace transform of given differential equation:
$$s^2Y(s)-sy(0)-y'(0)+Y(s)=0.5\frac{1}{s^2}$$
$$(s^2+1)Y(s)=\frac{0.5}{s^2}$$
$$Y(s)=\frac{0.5}{s^2(s^2+1)}=\frac{A}{s}+\frac{B}{s^2}+\frac{Cs+D}{s^2+1}$$
$$0.5=As(s^2+1)+B(s^2+1)+(Cs+D)s^2$$
$$0.5=As^3+As+Bs^2+B+Cs^3+Ds^2$$
$$0.5=s^3(A+C)+s^2(B+D)+sA+B$$
$$B=0.5$$
$$A=0$$
$$B+D=0\qqr D=-0.5$$
$$A+C=0\qqr C=0$$
Therefore the partial fractions are:
$$Y(s)=\frac{0}{s}+\frac{0.5}{s^2}+\frac{0s-0.5}{s^2+1}=\frac{0.5}{s^2}+\frac{-0.5}{s^2+1}$$
From Laplace transform table:
$$\mathcal{L}\{\sin(at)\}=\frac{a}{s^2+a^2}$$
The inverse laplace transform of $Y(s)$:
$$y(s)=0.5t-0.5\sin(t)$$
