\section{Several-Variables}

\subsection{Examples}
\subsubsection{Example 1: Gradient}
Find the rate of change of $f(x,y)=y^4+2xy^3+x^2y^2$ at $(0,1)$ in each of the following directions:
\begin{enumerate}
  \item $\mathbf{i}+2\mathbf{j}$
  \item $\mathbf{j}-2\mathbf{i}$
  \item $3\mathbf{i}$
  \item $\mathbf{i}+\mathbf{j}$
\end{enumerate}

\subsubsection{Example 2: Jacobian}
Find the Jacobian $Df(1,0)$ for the transformation from $\mathbb{R}^2$ to $\mathbb{R}^3$ given by:
$$\mathbf{f}(x,y)=(x e^{y}+\cos(\pi y)\,,x^{2},x-e^{y})$$

\subsubsection{Example 3: Chain Rule}
If $z=\sin(x^2y)$ where $x=st^2$ and $y=s^2+\frac{1}{t}$, find $\frac{\partial z}{\partial s}$ and $\frac{\partial z}{\partial t}$ using chain rule.

\rule{\textwidth}{0.5pt}

For: 
$${\frac{\partial z}{\partial s}}={\frac{\partial z}{\partial x}}{\frac{\partial x}{\partial s}}+{\frac{\partial z}{\partial y}}{\frac{\partial y}{\partial s}}$$
$${\frac{\partial z}{\partial x}}=2xy\cos(x^2y)$$
$${\frac{\partial x}{\partial s}}=t^2$$
$${\frac{\partial z}{\partial y}}=x^2\cos(x^2y)$$
$${\frac{\partial y}{\partial s}}=2s$$

Find:
$${\frac{\partial z}{\partial s}}=(2xy\cos(x^2y))t^2+(x^2\cos(x^2y))2s$$

Replace $x$ and $y$ with $x=st^2$ and $y=s^2+\frac{1}{t}$:
$$\frac{\partial z}{\partial s}=(4s^3t^4+2st^3)\cos(s^4t^4+s^2t^3)$$

Same principal for:
$${\frac{\partial z}{\partial t}}={\frac{\partial z}{\partial y}}{\frac{\partial y}{\partial t}}+{\frac{\partial z}{\partial y}}{\frac{\partial y}{\partial t}}$$


\subsubsection{Example 4: Substitution}
If $z=\sin(x^2y)$ where $x=st^2$ and $y=s^2+\frac{1}{t}$ find $\frac{\partial z}{\partial s}$ and $\frac{\partial z}{\partial t}$ using substitution.

\rule{\textwidth}{0.5pt}

$$z=\sin\left((st^2)^2s^2+\frac{1}{t}\right)=\sin\left(s^2t^4(s^2+\frac{1}{t})\right)=s^4t^4+s^2t^3$$
$$\frac{\partial z}{\partial s}=\sin(s^4t^4+s^2t^3)=(4s^3t^4+2st^3)\cos(s^4t^4+s^2t^3)$$
$$\frac{\partial z}{\partial t}=\sin(s^4t^4+s^2t^3)=(s^4 4t^3+s^2 3t^2)\cos(s^4t^4+s^2t^3)$$

\subsubsection{Example 5: Partial Differentiation}
Calculate $f_{223}(x,y,z)$, $f_{232}(x,y,z)$, and $f_{322}(x,y,z)$ of the following function:
$$f(x,y,z)=e^{x-2y+3z}$$

Normal Differentiation. For $f_{223}(x,y,z)$, start with $y$, then $y$ again, and then $z$:
$$\frac{\partial }{\partial z}\frac{\partial }{\partial y}\frac{\partial f(x,y,z)}{\partial y}$$
